armored/linear_search/scratch/check_assum.v
@@ -1,0 +1,4 @@
+Require Import exp5_term.
+Print Assumptions exec_a18.
+Check ls_instrs_a1c.
+Check bv_add_pc.
