armored/linear_search/scratch/probe_bvn.v
@@ -1,0 +1,9 @@
+From stdpp.bitvector Require Import definitions.
+Open Scope bv_scope.
+
+(* Can lazy unfold bvn_val/bvn_n on a bv_to_bvn constructor? *)
+Eval lazy in (bvn_val (bv_to_bvn (BV 64 0))).
+Eval lazy in (bvn_n (bv_to_bvn (BV 64 0))).
+Axiom t : bv 64.
+Eval lazy in (bvn_val (bv_to_bvn t)).
+Eval cbv in (bvn_val (bv_to_bvn (BV 64 0))).
