armored/linear_search/scratch/probe_e57.v
@@ -1,0 +1,27 @@
+From isla Require Import opsem.
+From stdpp.bitvector Require Import definitions.
+
+Open Scope bv_scope. Open Scope Z_scope.
+
+Definition e57_probe (i len : bv 64) : exp :=
+  Manyop Concat
+    [Manyop Concat
+       [Manyop Concat
+          [Manyop (Bvmanyarith Bvor)
+             [Manyop (Bvmanyarith Bvand)
+                [Val (Val_Bits (BV 1 0x0)) Mk_annot;
+                 Unop Bvnot (Val (Val_Bits (BV 1 0x1)) Mk_annot) Mk_annot] Mk_annot;
+              Unop (Extract 0 0)
+                (Binop (Bvarith Bvlshr)
+                   (Val (Val_Bits (bv_extract 0 64 (bv_add (bv_add (bv_zero_extend 128 i) (bv_zero_extend 128 (bv_not len))) (BV 128 1))))) Mk_annot)
+                   (Unop (Extract 63 0) (Val (Val_Bits (BV 128 0x3f))) Mk_annot) Mk_annot) Mk_annot] Mk_annot;
+           Ite (Binop Eq (Val (Val_Bits (bv_extract 0 64 (bv_add (bv_add (bv_zero_extend 128 i) (bv_zero_extend 128 (bv_not len))) (BV 128 1))))) (Val (Val_Bits (BV 64 0))) Mk_annot)
+             (Val (Val_Bits (BV 1 0x1)) Mk_annot) (Val (Val_Bits (BV 1 0x0)) Mk_annot) Mk_annot] Mk_annot;
+       Ite (Binop Eq (Unop (ZeroExtend 64) (Val (Val_Bits (bv_extract 0 64 (bv_add (bv_add (bv_zero_extend 128 i) (bv_zero_extend 128 (bv_not len))) (BV 128 1))))) Mk_annot)
+                      (Val (Val_Bits (bv_add (bv_add (bv_zero_extend 128 i) (bv_zero_extend 128 (bv_not len))) (BV 128 1)))) Mk_annot)
+         (Val (Val_Bits (BV 1 0x0)) Mk_annot) (Val (Val_Bits (BV 1 0x1)) Mk_annot) Mk_annot] Mk_annot;
+    Ite (Binop Eq (Unop (SignExtend 64) (Val (Val_Bits (bv_extract 0 64 (bv_add (bv_add (bv_zero_extend 128 i) (bv_zero_extend 128 (bv_not len))) (BV 128 1))))) Mk_annot)
+                  (Manyop (Bvmanyarith Bvadd) [Manyop (Bvmanyarith Bvadd) [Unop (SignExtend 64) (Val (Val_Bits i)) Mk_annot; Unop (SignExtend 64) (Val (Val_Bits (bv_not len))) Mk_annot] Mk_annot; Val (Val_Bits (BV 128 1)) Mk_annot] Mk_annot) Mk_annot)
+       (Val (Val_Bits (BV 1 0x0)) Mk_annot) (Val (Val_Bits (BV 1 0x1)) Mk_annot) Mk_annot] Mk_annot.
+
+Eval lazy [eval_exp eval_unop eval_manyop eval_binop bvn_to_bv bv_to_bvn] in (eval_exp (e57_probe i len)).
