armored/linear_search/scratch/probe_e57b.v
@@ -1,0 +1,45 @@
+From isla Require Import opsem.
+From stdpp.bitvector Require Import definitions.
+Import ListNotations.
+
+Open Scope bv_scope. Open Scope Z_scope.
+
+Parameter i len : bv 64.
+Parameter i_lt_len : (bv_unsigned i < bv_unsigned len)%Z.
+
+Definition a4_sum (i len : bv 64) : bv 128 :=
+  bv_add (bv_add (bv_zero_extend 128 i) (bv_zero_extend 128 (bv_not len))) (BV 128 1).
+Definition a4_res (i len : bv 64) : bv 64 := bv_extract 0 64 (a4_sum i len).
+
+Definition e57 (i len : bv 64) : exp :=
+  Manyop Concat
+    [ Manyop Concat
+        [ Manyop Concat
+            [ Manyop (Bvmanyarith Bvor)
+                [ Manyop (Bvmanyarith Bvand)
+                   [Val (Val_Bits (BV 1 0x0)) Mk_annot;
+                    Unop Bvnot (Val (Val_Bits (BV 1 0x1)) Mk_annot) Mk_annot] Mk_annot;
+                  Unop (Extract 0 0)
+                    (Binop (Bvarith Bvlshr)
+                       (Val (Val_Bits (a4_res i len)) Mk_annot)
+                       (Unop (Extract 63 0) (Val (Val_Bits (BV 128 0x3f)) Mk_annot) Mk_annot)
+                       Mk_annot) Mk_annot ] Mk_annot;
+              Ite (Binop Eq (Val (Val_Bits (a4_res i len)) Mk_annot)
+                     (Val (Val_Bits (BV 64 0)) Mk_annot) Mk_annot)
+                (Val (Val_Bits (BV 1 0x1)) Mk_annot)
+                (Val (Val_Bits (BV 1 0x0)) Mk_annot) Mk_annot ] Mk_annot;
+          Ite (Binop Eq (Unop (ZeroExtend 64) (Val (Val_Bits (a4_res i len)) Mk_annot) Mk_annot)
+                  (Val (Val_Bits (a4_sum i len)) Mk_annot) Mk_annot)
+            (Val (Val_Bits (BV 1 0x0)) Mk_annot)
+            (Val (Val_Bits (BV 1 0x1)) Mk_annot) Mk_annot ] Mk_annot;
+      Ite (Binop Eq (Unop (SignExtend 64) (Val (Val_Bits (a4_res i len)) Mk_annot) Mk_annot)
+              (Manyop (Bvmanyarith Bvadd)
+                 [ Manyop (Bvmanyarith Bvadd)
+                     [ Unop (SignExtend 64) (Val (Val_Bits i) Mk_annot) Mk_annot;
+                       Unop (SignExtend 64) (Val (Val_Bits (bv_not len)) Mk_annot) Mk_annot ] Mk_annot;
+                   Val (Val_Bits (BV 128 1)) Mk_annot ] Mk_annot) Mk_annot)
+        (Val (Val_Bits (BV 1 0x0)) Mk_annot)
+        (Val (Val_Bits (BV 1 0x1)) Mk_annot) Mk_annot ] Mk_annot.
+
+Eval lazy [eval_exp eval_unop eval_manyop eval_binop bvn_to_bv bvn_val bvn_n] in
+  (eval_exp (e57 i len)).
