armored/linear_search/scratch/probe_eval.v
@@ -1,0 +1,19 @@
+From isla Require Import opsem.
+From stdpp.bitvector Require Import definitions.
+
+Open Scope bv_scope. Open Scope Z_scope.
+
+Check eval_binop.
+Check eval_manyop.
+
+Example t1 (i : bv 64) :
+  eval_binop Eq
+    (bvn_of (bv_extract 0 64 (bv_add (bv_add (bv_zero_extend 128 i) (bv_zero_extend 128 (bv_not (BV 64 16)))) (BV 128 1))))
+    (bvn_of (BV 64 0)) = Some (Val_Bool true).
+Proof. lazy [eval_binop bvn_to_bv]. vm_compute. Admitted.
+
+Example t2 (i : bv 64) :
+  eval_binop Eq
+    (bvn_of (bv_extract 0 64 (bv_add (bv_add (bv_zero_extend 128 i) (bv_zero_extend 128 (bv_not (BV 64 16)))) (BV 128 1))))
+    (bvn_of (BV 64 0)) = Some (Val_Bool (bool_decide (bv_unsigned (bv_extract 0 64 (bv_add (bv_add (bv_zero_extend 128 i) (bv_zero_extend 128 (bv_not (BV 64 16)))) (BV 128 1))) = bv_unsigned (BV 64 0)))).
+Proof. lazy [eval_binop bvn_to_bv]. reflexivity. Qed.
