armored/linear_search/scratch/probe_eval2.v
@@ -1,0 +1,30 @@
+From isla Require Import opsem.
+From stdpp.bitvector Require Import definitions.
+
+Open Scope bv_scope. Open Scope Z_scope.
+
+Check bv_to_bvn.
+
+Example t2 (i : bv 64) :
+  eval_exp (Ite
+      (Binop Eq
+        (Val (Val_Bits (bv_extract 0 64 (bv_add (bv_add (bv_zero_extend 128 i) (bv_zero_extend 128 (bv_not (BV 64 16)))) (BV 128 1)))))
+        (Val (Val_Bits (BV 64 0))))
+      (Val (Val_Bits (BV 1 1)))
+      (Val (Val_Bits (BV 1 0)))) = Some (Val_Bits (BV 1 1)).
+Proof.
+  lazy [eval_exp eval_binop bvn_to_bv bool_decide Decidable.decide decide]. 
+  reflexivity.
+Fail Qed.
+Abort.
+
+Example t2b (i : bv 64) :
+  eval_exp (Ite
+      (Binop Eq
+        (Val (Val_Bits (bv_extract 0 64 (bv_add (bv_add (bv_zero_extend 128 i) (bv_zero_extend 128 (bv_not (BV 64 16)))) (BV 128 1)))))
+        (Val (Val_Bits (BV 64 0))))
+      (Val (Val_Bits (BV 1 1)))
+      (Val (Val_Bits (BV 1 0)))) = None.
+Proof.
+  lazy [eval_exp eval_binop bvn_to_bv]. reflexivity.
+Qed.
