armored/linear_search/scratch/probe_eval3.v
@@ -1,0 +1,17 @@
+From isla Require Import opsem.
+From stdpp.bitvector Require Import definitions.
+
+Open Scope bv_scope. Open Scope Z_scope.
+
+Check eval_exp.
+
+Example t2b (i : bv 64) :
+  eval_exp (Ite
+      (Binop Eq
+        (Val (Val_Bits (bv_extract 0 64 (bv_add (bv_add (bv_zero_extend 128 i) (bv_zero_extend 128 (bv_not (BV 64 16)))) (BV 128 1)))) Mk_annot)
+        (Val (Val_Bits (BV 64 0)) Mk_annot) Mk_annot)
+      (Val (Val_Bits (BV 1 1)) Mk_annot)
+      (Val (Val_Bits (BV 1 0)) Mk_annot) Mk_annot) = None.
+Proof.
+  lazy [eval_exp eval_binop bvn_to_bv]. reflexivity.
+Qed.
