armored/linear_search/scratch/probe_lazy.v
@@ -1,0 +1,34 @@
+From Coq.ssr Require Import ssreflect.
+From stdpp Require Import prelude gmap.
+From stdpp.bitvector Require Import definitions.
+Require Import isla.opsem.
+
+Open Scope N_scope.
+Open Scope Z_scope.
+
+Ltac ls_lazy :=
+  lazy [eval_exp mapM mbind option_bind eval_unop eval_manyop eval_binop option_fmap option_map fmap mret option_ret guard_or mthrow option_mfail foldl bvn_to_bv bvn_n bvn_val bv_unsigned decide decide_rel BinNat.N.eq_dec N.eq_dec N_rec N_rect N.add N.mul N.sub Pos.add Pos.mul Pos.succ Pos.pred Pos.sub_mask Pos.double_mask Pos.succ_double_mask Pos.pred_double Pos.double_pred_mask].
+
+Lemma probe_lazy_evar :
+  forall (i : bv 64),
+  eval_exp (Manyop (Bvmanyarith Bvadd)
+      [Unop (Extract 63 0) (Unop (ZeroExtend 64) (Val (Val_Bits (bv_to_bvn i)) Mk_annot) Mk_annot) Mk_annot;
+       Val (Val_Bits (bv_to_bvn (BV 64 1))) Mk_annot] Mk_annot)
+  = Some (Val_Bits (bv_to_bvn (bv_add (bv_extract 0 64 (bv_zero_extend 128 i)) (BV 64 1)))).
+Proof.
+  move => i.
+  ls_lazy.
+  reflexivity.
+Qed.
+
+Lemma probe_lazy_goal_evar (i : bv 64) :
+  let e := bv_to_bvn i in
+  eval_exp (Manyop (Bvmanyarith Bvadd)
+      [Unop (Extract 63 0) (Unop (ZeroExtend 64) (Val (Val_Bits e)) Mk_annot) Mk_annot;
+       Val (Val_Bits (bv_to_bvn (BV 64 1))) Mk_annot] Mk_annot)
+  = Some (Val_Bits (bv_to_bvn (bv_add (bv_extract 0 64 (bv_zero_extend 128 i)) (BV 64 1)))).
+Proof.
+  move => e.
+  ls_lazy.
+  reflexivity.
+Qed.
