armored/linear_search/scratch/probe_lseval.v
@@ -1,0 +1,46 @@
+From Coq.ssr Require Import ssreflect.
+From stdpp Require Import prelude gmap.
+From stdpp.bitvector Require Import definitions.
+Require Import isla.opsem.
+
+Open Scope N_scope.
+Open Scope Z_scope.
+
+Lemma probe_concrete :
+  eval_exp (Manyop (Bvmanyarith Bvadd)
+      [Unop (Extract 63 0) (Unop (ZeroExtend 64) (Val (Val_Bits (BV 64 42)) Mk_annot) Mk_annot) Mk_annot;
+       Val (Val_Bits (BV 64 1)) Mk_annot] Mk_annot)
+  = Some (Val_Bits (bv_add (bv_extract 0 64 (bv_zero_extend 64 (BV 64 42))) (BV 64 1))).
+Proof.
+  time "cbn" cbn.
+  reflexivity.
+Qed.
+
+Lemma probe_variable (i : bv 64) :
+  eval_exp (Manyop (Bvmanyarith Bvadd)
+      [Unop (Extract 63 0) (Unop (ZeroExtend 64) (Val (Val_Bits i) Mk_annot) Mk_annot) Mk_annot;
+       Val (Val_Bits (BV 64 1)) Mk_annot] Mk_annot)
+  = Some (Val_Bits (bv_add (bv_extract 0 64 (bv_zero_extend 64 i)) (BV 64 1))).
+Proof.
+  time "refl" reflexivity.
+Qed.
+
+Lemma probe_variable_vm (i : bv 64) :
+  eval_exp (Manyop (Bvmanyarith Bvadd)
+      [Unop (Extract 63 0) (Unop (ZeroExtend 64) (Val (Val_Bits i) Mk_annot) Mk_annot) Mk_annot;
+       Val (Val_Bits (BV 64 1)) Mk_annot] Mk_annot)
+  = Some (Val_Bits (bv_add (bv_extract 0 64 (bv_zero_extend 64 i)) (BV 64 1))).
+Proof.
+  time "vm" vm_compute.
+  reflexivity.
+Qed.
+
+Lemma probe_evar :
+  eval_exp (Manyop (Bvmanyarith Bvadd)
+      [Unop (Extract 63 0) (Unop (ZeroExtend 64) (Val (Val_Bits ?e) Mk_annot) Mk_annot) Mk_annot;
+       Val (Val_Bits (BV 64 1)) Mk_annot] Mk_annot)
+  = Some (Val_Bits (bv_add (bv_extract 0 64 (bv_zero_extend 64 ?e)) (BV 64 1))).
+Proof.
+  time "vm-evar" vm_compute.
+  reflexivity.
+Qed.
