armored/linear_search/scratch/probe_pc.v
@@ -1,0 +1,14 @@
+Require Import Coq.ZArith.ZArith.
+From stdpp.bitvector Require Import definitions.
+From stdpp.bitvector Require Import tactics.
+From isla.instructions.linear_search Require Import instrs.
+Open Scope bv_scope.
+Local Open Scope Z_scope.
+
+Lemma t6 : ls_instrs !! (BV 64 0x1030001c) = Some (a1c).
+Proof. reflexivity. Qed.
+
+Lemma bv_add_solve : bv_add (BV 64 0x10300018) (BV 64 4) = BV 64 0x1030001c.
+Proof.
+  apply bv_eq. simpl. lia.
+Qed.
