armored/linear_search/scratch/probe_vmvar.v
@@ -1,0 +1,17 @@
+From Coq.ssr Require Import ssreflect.
+From stdpp Require Import prelude gmap.
+From stdpp.bitvector Require Import definitions.
+Require Import isla.opsem.
+
+Open Scope N_scope.
+Open Scope Z_scope.
+
+Lemma probe_variable_vm (i : bv 64) :
+  eval_exp (Manyop (Bvmanyarith Bvadd)
+      [Unop (Extract 63 0) (Unop (ZeroExtend 64) (Val (Val_Bits (bv_to_bvn i)) Mk_annot) Mk_annot) Mk_annot;
+       Val (Val_Bits (bv_to_bvn (BV 64 1))) Mk_annot] Mk_annot)
+  = Some (Val_Bits (bv_to_bvn (bv_add (bv_extract 0 64 (bv_zero_extend (64 + 64) i)) (BV 64 1)))).
+Proof.
+  vm_compute.
+  reflexivity.
+Qed.
